write some functions

HOL_To_IMP_Minus/Refinements/HOL_To_IMP_Minus_Datatypes.thy
@@ -2,12 +2,62 @@
 theory HOL_To_IMP_Minus_Datatypes
   imports
     HOL_To_IMP_Minus_Arithmetics
+    "HOL-Data_Structures.Cmp"
 begin
+
+datatype_compile_nat cmp_val
 
 locale HOL_To_HOL_Nat =
   notes transport_eq_id.partial_equivalence_rel_equivalenceI[per_intro del]
   and transport_eq_restrict_id.partial_equivalence_rel_equivalence[per_intro del]
 begin
+
+section \<open>Pairs\<close>
+
+function_compile_nat fst_def
+function_compile_nat snd_def
+
+section\<open>Three-way compare\<close>
+
+(* function_compile_nat cmp_def *)
+
+section\<open>Lists\<close>
+
+paragraph \<open>length\<close>
+
+(*
+fun length_aux :: "nat \<Rightarrow> 'a list \<Rightarrow> nat" where
+  "length_aux acc [] = acc" |
+  "length_aux acc (_ # xs) = length_aux (Suc acc) xs"
+
+
+fun length :: "'a list \<Rightarrow> nat" where
+  "length [] = 0" |
+  "length (_ # xs) = Suc (length xs)"
+
+lemma "List.length xs = local.length xs" by (induction xs) auto
+
+case_of_simps length_eq : length.simps
+function_compile_nat length_eq
+*)
+
+lemma length_eq: "length xs = (case xs of [] \<Rightarrow> 0 | (_ # xs') \<Rightarrow> Suc (length xs'))"
+  by (simp add: list.case_eq_if)
+
+function_compile_nat length_eq
+print_theorems
+
+paragraph\<open>compare_lengths\<close>
+
+fun compare_lengths :: "'a list \<Rightarrow> 'b list \<Rightarrow> cmp_val" where
+  "compare_lengths [] [] = EQ" |
+  "compare_lengths [] _ = LT" |
+  "compare_lengths _ [] = GT" |
+  "compare_lengths (_ # xs) (_ # ys) = compare_lengths xs ys"
+
+case_of_simps compare_lengths_eq : compare_lengths.simps
+
+function_compile_nat compare_lengths_eq
 
 paragraph \<open>rev\<close>
 
@@ -32,9 +82,36 @@ function_compile_nat zip_eq
 
 end
 
-
 context HOL_To_IMP_Minus
 begin
+
+section \<open>Pairs\<close>
+
+compile_nat Pair_nat_def
+HOL_To_IMP_Minus_correct Pair_nat by cook
+
+lemmas fst_nat_eq_unfolded = HOL_To_HOL_Nat.fst_nat_eq_unfolded[simplified case_prod_nat_def]
+unconditional_nat fst_nat_eq_unfolded
+compile_nat fst_nat_unconditional.simps
+HOL_To_IMP_Minus_correct fst_nat_unconditional by cook
+
+lemmas snd_nat_eq_unfolded = HOL_To_HOL_Nat.snd_nat_eq_unfolded[simplified case_prod_nat_def]
+unconditional_nat snd_nat_eq_unfolded
+compile_nat snd_nat_unconditional.simps
+HOL_To_IMP_Minus_correct snd_nat_unconditional by cook
+
+section \<open>Three-way compare\<close>
+
+compile_nat LT_nat_def
+HOL_To_IMP_Minus_correct LT_nat by cook
+
+compile_nat EQ_nat_def
+HOL_To_IMP_Minus_correct EQ_nat by cook
+
+compile_nat GT_nat_def
+HOL_To_IMP_Minus_correct GT_nat by cook
+
+section\<open>Lists\<close>
 
 compile_nat Cons_nat_def
 HOL_To_IMP_Minus_correct Cons_nat by cook
@@ -42,16 +119,47 @@ HOL_To_IMP_Minus_correct Cons_nat by cook
 compile_nat Nil_nat_def
 HOL_To_IMP_Minus_correct Nil_nat by cook
 
-thm HOL_To_HOL_Nat.rev_aux_nat_eq_unfolded
+paragraph \<open>length\<close>
+
+(* TODO: these all end up getting named size_... *)
+thm HOL_To_HOL_Nat.size_nat_eq_unfolded
+lemmas size_nat_eq = HOL_To_HOL_Nat.size_nat_eq_unfolded[simplified case_list_nat_def]
+unconditional_nat size_nat_eq
+compile_nat size_nat_unconditional.simps
+(* TODO: also the proof doesn't work *)
+(* HOL_To_IMP_Minus_correct size_nat_unconditional by (cook mode = tailcall) *)
+
+paragraph\<open>compare_lengths\<close>
+
+lemmas compare_lengths_nat_eq = HOL_To_HOL_Nat.compare_lengths_nat_eq_unfolded[simplified case_list_nat_def]
+unconditional_nat compare_lengths_nat_eq
+declare compare_lengths_nat_unconditional.simps [simp del]
+compile_nat compare_lengths_nat_unconditional.simps
+HOL_To_IMP_Minus_correct compare_lengths_nat_unconditional by (cook mode = tailcall)
+
+paragraph \<open>rev\<close>
+
 lemmas rev_aux_nat_eq = HOL_To_HOL_Nat.rev_aux_nat_eq_unfolded[simplified case_list_nat_def]
 unconditional_nat rev_aux_nat_eq
+declare rev_aux_nat_unconditional.simps [simp del]
 compile_nat rev_aux_nat_unconditional.simps
+HOL_To_IMP_Minus_correct rev_aux_nat_unconditional by (cook mode = tailcall)
 
 (*
+TODO: can't do functions with helpers!
 thm HOL_To_HOL_Nat.rev_nat_eq_unfolded
 lemmas rev_nat_eq = HOL_To_HOL_Nat.rev_nat_eq_unfolded[simplified case_list_nat_def]
 unconditional_nat rev_nat_eq
 *)
+
+paragraph \<open>zip\<close>
+
+lemmas zip_nat_eq = HOL_To_HOL_Nat.zip_nat_eq_unfolded[simplified case_list_nat_def]
+unconditional_nat zip_nat_eq
+declare zip_nat_unconditional.simps [simp del]
+compile_nat zip_nat_unconditional.simps
+(* TODO: proof fails *)
+(* HOL_To_IMP_Minus_correct zip_nat_unconditional by (cook mode = tailcall) *)
 
 end
 
